Making progress on const fold proof

theories/const.v
@@ -3,10 +3,12 @@ Require Import Coq.Program.Wf.
 Require Import FunInd.
 Require Import Lia.
 Require Import Coq.Program.Tactics.
+From Coq Require Import FMaps.
 
 From Equations Require Import Equations.
 
 Import CPS.
+Open Scope cps_scope.
 
 (** [in_map l f] is just like [map f l] except that the function carries a proof
     that its argument is an element of [l]. *)
@@ -73,8 +75,13 @@ Next Obligation. simpl. rewrite Nlt_succ_le. apply list_max_in. apply List.in_ma
 assumption. 
 Defined.
 
-
-Definition matches s_1 s_2 := s_1.(tr) = s_2.(tr).
+Definition tr_matches src opt := src.(tr) = opt.(tr).
+Definition st_matches src opt := forall f src_bod args,
+    Some (args, src_bod) = FnMap.find f src.(fstor) ->
+    exists opt_bod,
+    Some (args, opt_bod) = FnMap.find f opt.(fstor) /\
+        opt_bod = const_fold src_bod.
+                            
 
 Fixpoint const_fold_fuel (exp: cexp) (fuel: nat): cexp :=
     match (fuel, exp) with
@@ -104,7 +111,7 @@ Qed.
 
 
 
-Theorem const_fuel_lock_single: forall c c' s_1 s_2 s_1' n,
+(* Theorem const_fuel_lock_single: forall c c' s_1 s_2 s_1' n,
     matches s_1 s_2 -> small_step c s_1 c' s_1' -> n > depth c ->
     (exists c_2' s_2', small_step (const_fold_fuel c n) s_2 c_2' s_2' /\ matches s_1' s_2').
 Proof.
@@ -119,15 +126,31 @@ Proof.
     - assumption.
     (* Effect *)
     - unfold matches. unfold matches in H. now rewrite H.
-Qed.    
+Qed.     *)
 
-Lemma const_lock_single: forall c c' s_1 s_2 s_1',
-    matches s_1 s_2 -> small_step c s_1 c' s_1' ->
-    (exists c_2' s_2', small_step (const_fold c) s_2 c_2' s_2' /\ matches s_1' s_2').
+(* Lemma const_lock_single: forall c c' s_1 s_2 s_1',
+    st_matches s_1 s_2 -> tr_matches s_1 s_2 -> small_step c s_1 c' s_1' ->
+    (exists c_2' s_2', small_step (const_fold c) s_2 c_2' s_2' 
+        /\ st_matches s_1' s_2' /\ tr_matches s_1' s_2').
 Proof.
-    intros. destruct H0.
-    all: eexists; eexists; split; (assumption || autorewrite with const_fold; simpl; auto).
+    intros. destruct H1.
+    all: unfold st_matches in H; unfold tr_matches in H0; eexists; eexists; split; (assumption || autorewrite with const_fold; simpl; auto).
     (* Select *)
+    - apply sapp.
+        + autorewrite with const_fold. unfold st_matches in H. unfold tr_matches in H0.
+            * now rewrite in_map_length.
+            * assumption.
+        + split.
+            * unfold st_matches. intros. specialize H with (f := f) (src_bod := src_bod) (args := args).
+                destruct H. split.
+                -- now rewrite H.
+                -- apply H0.
+            * unfold tr_matches. unfold tr_matches in H1. now rewrite H1.
+    (* Select case 2 *) 
+    - unfold matches in H. destruct H. rewrite H. unfold matches; split.
+        + destruct fns; trivial. 
+        + apply H0.
+    (* Select case 2 *)
     - autorewrite with const_fold. apply ssel. destruct H0. split.
         * now rewrite in_map_length.
         * assumption.
@@ -135,10 +158,10 @@ Proof.
     - assumption.
     (* Effect *)
     - unfold matches. unfold matches in H. now rewrite H.
-Qed.
+Qed. *)
 
 (* I don't think this is right... *)
-Inductive lock_matches: cexp -> State -> cexp -> State -> Prop :=
+(* Inductive lock_matches: cexp -> State -> cexp -> State -> Prop :=
     | lock_matches_intro: forall c_1 s_1 c_2 s_2, 
         matches s_1 s_2 -> 
         c_2 = const_fold c_1 -> 
@@ -148,10 +171,158 @@ Inductive lock_matches: cexp -> State -> cexp -> State -> Prop :=
         small_step c_1 s_1 c_1' s_1' ->
         small_step c_2 s_2 c_2' s_2' ->
         matches s_1' s_2' ->
-        lock_matches c_1' s_1' c_2' s_2'.
+        lock_matches c_1' s_1' c_2' s_2'. *)
 
-(* Or this... *)
-Theorem const_lock_simulation: forall c_1 s_1 c_1' s_1' c_2 s_2,
+Theorem const_fold_sub: forall op lhs rhs k,
+    const_fold (substitute O (i64 (bop_eval op lhs rhs)) k) =
+    substitute O (i64 (bop_eval op lhs rhs)) 
+        (const_fold (substitute O (i64 (bop_eval op lhs rhs)) k)).
+Proof.
+    Admitted.
+
+Theorem const_fold_app: forall f_body f_params args,
+    const_fold (apply_args f_body f_params args) = apply_args (const_fold f_body) f_params args.
+Proof.
+    Admitted.
+
+Inductive First {A B C} : (A * B * C) -> list (A * B * C) -> Prop :=
+    | First_hd : forall x xs, First x (x :: xs)
+    | First_tl : forall a1 a2 a3 b1 b2 b3 tl, a1 <> b1 -> 
+        First (a1, a2, a3) tl -> First (a1, a2, a3) ((b1, b2, b3) :: tl).
+
+Lemma first_implies_in: forall A B C (e: A * B * C) l, First e l -> In e l.
+Proof.
+    intros. induction H.
+    - apply in_eq.
+    - apply in_cons. assumption.
+Qed.
+
+Lemma first_append_map_fns: forall f args src_bod fns st (fn : cexp -> cexp),
+    First (f, args, src_bod) fns -> 
+    (FnMap.find f 
+        (append_fns (in_map fns (fun e _ => let '(a, b, _) := e in
+            (a, b, fn (snd e)))) st) = Some (args, fn src_bod)).
+Proof.
+    intros. remember (f, args, src_bod) as e. induction H.
+    - autorewrite with in_map. destruct x. destruct p. simpl.
+        inversion Heqe. apply FMFact.add_eq_o. reflexivity.
+    - autorewrite with in_map. simpl. rewrite FMFact.add_neq_o.
+        + apply IHFirst. now inversion Heqe.
+        + unfold "<>". intros Heq. inversion Heqe as (Heq1).
+            assert (a1 = b1) by (rewrite Heq; rewrite Heq1; reflexivity).
+            contradiction.
+Qed.
+
+Theorem find_append_map: forall k l s ra rb,
+    Some (ra, rb) = FnMap.find k (append_fns l s) ->
+    (Some (ra, rb) = FnMap.find k s /\ forall ra' rb', ~ In (k, ra', rb') l)
+        \/ First (k, ra, rb) l.
+Proof.
+    intros. induction l.
+    - simpl in H. left. split; auto.
+    - simpl in H. destruct a. destruct p. destruct (String.eqb k s0) eqn: H'.
+        + apply String.eqb_eq in H'. right. rewrite H' in H.
+            rewrite FMFact.add_eq_o in H. inversion H. rewrite H'. apply First_hd. 
+            reflexivity.
+        + apply String.eqb_neq in H'. rewrite FMFact.add_neq_o in H.
+            * apply IHl in H. destruct H.
+                -- left. destruct H. split; auto. unfold "~". intros.
+                    inversion H1.
+                    ++ apply H'. now inversion H2. 
+                    ++ now apply H0 in H2.
+                -- right. apply First_tl; assumption.
+            * unfold "<>" in *. intros. destruct H'. auto.
+Qed.
+
+Lemma not_in_append: forall f st l,
+    (forall a b, ~ In (f, a, b) l) -> FnMap.find f (append_fns l st) = FnMap.find f st.
+Proof. 
+    intros f st l. induction l.
+    - intros. now simpl.
+    - intros. simpl. destruct a. destruct p.
+        pose proof H as H'. specialize H with (a := n) (b := c).
+        unfold "~" in H.
+        assert (f <> k).
+        { unfold "<>". intros. apply H. rewrite H0. apply in_eq. }
+        rewrite FMFact.add_neq_o.
+        +  apply IHl. unfold "~". intros a b H''.
+            apply in_cons with (a := (k, n, c)) in H''.
+            now apply H' in H''.
+        + unfold "<>" in *. intros H1. apply eq_sym in H1.
+            now apply H0.
+Qed.
+
+Lemma in_map_nil: forall A B (l: list A) (f: forall (a: A), In a l -> B), 
+    in_map l f = nil <-> l = nil.
+Proof.
+    intros A B l. split.
+    - intros. destruct l.
+        + trivial.
+        + discriminate.
+    - intros. generalize dependent f. rewrite H. intros. now autorewrite with in_map.
+Qed.
+
+Lemma in_cons_neq: forall A B C (f s: A) (a c: B) (b d: C) (l: list (A * B * C)),
+    f <> s -> In (f, a, b) ((s, c, d) :: l) <-> In (f, a, b) l.
+Proof.
+    intros. split. 
+    - intros. destruct H0.
+        + inversion H0. apply eq_sym in H2. contradiction.
+        + assumption.
+    - intros. now apply in_cons. 
+Qed. 
+
+
+Theorem const_fold_step: forall c s c' s' s_2,
+    c @ s --> c' @ s' -> st_matches s s_2 -> tr_matches s s_2 -> exists s'', 
+        (const_fold c) @ s_2 --> (const_fold c') @ s'' /\ st_matches s' s'' /\ tr_matches s' s''.
+Proof.
+    intros. destruct H.
+    - eexists ?[s'']. split.
+        + autorewrite with const_fold. rewrite const_fold_sub at 2. now apply sbop.
+        + split; assumption.
+    - admit. (*Same idea as prev*)
+    - autorewrite with const_fold. unfold st_matches in H0. unfold tr_matches in H1.
+      pose proof H as H'. apply H0 in H. case H; intros. destruct H2.
+      exists s_2. split. 
+        + rewrite const_fold_app. rewrite <- H3. apply sapp. assumption.
+        + unfold st_matches. unfold tr_matches. split; assumption.
+    - autorewrite with const_fold. 
+        exists {| tr := tr s_2; fstor := append_fns (in_map fns (fun e _ => 
+            let '(a, b, _) := e in (a, b, const_fold (snd e)))) s_2.(fstor) |}.
+        split.
+        + apply sfix.
+        + split.
+            * unfold st_matches. simpl. intros f src_bod args H.
+                apply find_append_map in H. destruct H.
+                -- destruct H. unfold st_matches in H0.
+                    pose proof H as H'. apply H0 in H.
+                    rewrite not_in_append.
+                    ++ auto.
+                    ++ induction fns.
+                        ** unfold "~". intros. destruct H3; auto.
+                        ** simpl in *. autorewrite with in_map in *. destruct a. destruct p.
+                            assert (H3: ((forall ra' rb', (s, n, c) <> (f, ra', rb')) /\ 
+                                (forall ra' rb', ~ In (f, ra', rb') fns))).
+                            { 
+                                split; intros; specialize H2 with (ra' := ra') (rb' := rb');
+                                tauto. 
+                            } 
+                            destruct H3.
+                            assert (H5: s <> f).
+                            {
+                              specialize H3 with (ra' := n) (rb' := c).
+                              unfold "<>". intros. rewrite H5 in H3. now apply H3.
+                            }
+                            unfold "~". intros.
+                            apply IHfns with (a := a) (b := b) in H4.
+                            apply H4. rewrite in_cons_neq in H6; (auto || tauto).
+                -- rewrite first_append_map_fns with (args := args) (src_bod := src_bod) by assumption. 
+                    exists (const_fold src_bod). split; trivial.
+            * 
+Admitted.
+                    
+(* Theorem const_lock_simulation: forall c_1 s_1 c_1' s_1' c_2 s_2,
     lock_matches c_1 s_1 c_2 s_2 -> small_step c_1 s_1 c_1' s_1' -> 
     (exists c_2' s_2', small_step c_2 s_2 c_2' s_2' /\ lock_matches c_1' s_1' c_2' s_2').
 Proof.
@@ -170,4 +341,4 @@ Proof.
         rewrite <- H2 in H0. exists c_2'. exists s_2'. split.
         + apply H0.
         + apply lock_matches_step with (c_1 := c_1) (s_1 := s_1) (c_2 := c_2) (s_2 := s_2); auto.
-    -  *)
+    -  *) *)
